regex/Regex/Syntax/Ast.lean
@@ -16,7 +16,7 @@ inductive Ast : Type where
   | group : Ast → Ast
   | alternate : Ast → Ast → Ast
   | concat : Ast → Ast → Ast
-  | repeat : Nat → Option Nat → Ast → Ast
+  | repeat : Nat → Option Nat → Bool → Ast → Ast
   | classes : Classes → Ast
   | perl : PerlClass → Ast
   | dot : Ast
@@ -29,18 +29,20 @@ where
     | 0 => accum
     | n + 1 => go (.concat accum e) n
 
-def applyRepetitions (min : Nat) (max : Option Nat) (e : Expr) : Expr :=
+def applyRepetitions (min : Nat) (max : Option Nat) (greedy : Bool) (e : Expr) : Expr :=
   match min, max with
-  | 0, .some 1 => .alternate e .epsilon
-  | 0, .none => .star e
-  | 1, .none => .concat e (.star e)
-  | min, .none => .concat (repeatConcat e min) (.star e)
+  | 0, .some 1 => if greedy then .alternate e .epsilon else .alternate .epsilon e
+  | 0, .none => .star greedy e
+  | 1, .none => .concat e (.star greedy e)
+  | min, .none => .concat (repeatConcat e min) (.star greedy e)
   | 0, .some max =>
     if max == 0 then .epsilon
     else repeatConcat (.alternate e .epsilon) max
   | min, .some max =>
     if min == max then repeatConcat e min
-    else .concat (repeatConcat e min) (repeatConcat (.alternate e .epsilon) (max - min))
+    else
+      let e' := if greedy then .alternate e .epsilon else .alternate .epsilon e
+      .concat (repeatConcat e min) (repeatConcat e' (max - min))
 
 def Ast.toRegexAux (index : Nat) (ast : Ast) : Nat × Expr :=
   match ast with
@@ -59,9 +61,9 @@ def Ast.toRegexAux (index : Nat) (ast : Ast) : Nat × Expr :=
     let (index₁, r₁) := h₁.toRegexAux index
     let (index₂, r₂) := h₂.toRegexAux index₁
     (index₂, .concat r₁ r₂)
-  | .repeat min max h =>
+  | .repeat min max greedy h =>
     let (index', r) := h.toRegexAux index
-    (index', applyRepetitions min max r)
+    (index', applyRepetitions min max greedy r)
   | .classes cs => (index, .classes cs)
   | .perl pc => (index, .classes ⟨false, #[Class.perl pc]⟩)
   | .dot => (index, .classes ⟨false, #[Class.beforeLineBreak, Class.afterLineBreak]⟩)
